\newgeometry{left=.3cm,right=1.5cm,bottom=.5cm}

\section{Formulas}
\label{formulas}

\ \\[0mm]

\noindent%
\begin{minipage}[l]{0.32\textwidth}
\noindent%
\textbf{Descriptive~Statistics}
\begin{align*}
&\bar{x} =\frac{\sum{x_i}}{n} \\[3.5mm]
&s_x = \sqrt{\frac{1}{n-1}\sum{(x_i-\bar{x})^2}} \\[3.5mm]
&r = \frac{1}{n-1}
    \sum{\Big(\frac{x_i-\bar{x}}{s_x}\Big)
    \Big(\frac{y_i-\bar{y}}{s_y}\Big)} \\[3.5mm]
&\hat{y} = b_0+b_1x \\[3.5mm]
&b_0 = \bar{y}-b_1\bar{x} \\[3.5mm]
&b_1 = r\frac{s_y}{s_x} \\[3.5mm]
&s_{b_1}
    = \frac{\sqrt{\frac{\sum{(y_i-\hat{y}_i)^2}}{n-2}}}
        {\sqrt{\sum{(x_i-\bar{x})^2}}}
\end{align*}
\ \vspace{11mm}

\ 
\end{minipage}
\begin{minipage}[l]{0.13\textwidth}
\ 
\end{minipage}
\begin{minipage}[l]{0.35\textwidth}
\noindent%
\textbf{Probability}
\begin{align*}
&P(A \cup B) = P(A) + P(B) - P(A\cap B) \\[2.5mm]
&P(A | B) = \frac{P(A \cap B)}{P(B)} \\[2.5mm]
&E(X)=\mu_x=\sum{(x_i\times p_i)} \\[2.5mm]
&Var(X) = \sigma_x^2=\sum{((x_i-\mu_x)^2\times p_i)} \\[2.5mm]
&\mu_{\bar{x}}
    = \mu \qquad \quad
        \ \sigma_{\bar{x}} = \frac{\sigma}{\sqrt{n}} \\[8mm]
&\text{If $X$ has a binomial distribution with} \\
&\text{parameters $n$ and $p$, then:} \\[2.5mm]
&P(X=k)={n\choose k} p^k(1-p)^{n-k} \\[2.5mm]
&\mu_x=np \qquad \quad  \ \sigma_x=\sqrt{np(1-p)} \\[2.5mm]
&\mu_{\hat{p}}
    = p\qquad \qquad
        \small{\sigma_{\hat{p}}=\sqrt{\frac{p(1-p)}{n}}}
\end{align*}
\end{minipage} \\[10mm]

\noindent%
\textbf{Inferential~Statistics} \vspace{4mm}

$$\text{standardized test statistic: }  \frac{\text{point estimate} - \text{null value}}{SE \text{ of estimate}}\qquad\ $$
$$\text{confidence interval: } \text{point estimate} \ \pm \ \text{critical value}\times SE \text{ of estimate}\qquad\ $$
\\[2mm]

\noindent%
\begin{tabular}{lcccl}
&parameter & point estimate &$SE$  of estimate& \\
single proportion &$p$ &$\hat{p}$ &$\sqrt{\frac{\hat{p}(1-\hat{p})}{n}}$ &
    {\footnotesize when $H_0$: $p=p_0$, use $\sqrt{\frac{p_0(1-p_0)}{n}}$} \\
\\
diff.~of proportions &
    $p_1-p_2$ & $\hat{p}_1-\hat{p}_2$ &
    $\sqrt{\frac{\hat{p}_1(1-\hat{p}_1)}{n_1}+
        \frac{\hat{p}_2(1-\hat{p}_2)}{n_2}}$ &
    {\footnotesize when $H_0$: $p_1=p_2$, use $\scriptscriptstyle{\sqrt{\hat{p}(1-\hat{p})}\sqrt{\frac{1}{n_1}+\frac{1}{n_2}}}$}
    \\
single mean & $\mu$ & $\bar{x}$ & $\frac{s}{\sqrt{n}}$&\quad  \\
\\
mean of differences& $\mu_{\text{\emph{diff}}}$ & $\bar{x}_{\text{\emph{diff}}}$ & $\frac{s_{\text{\emph{diff}}}}{\sqrt{n_{\text{\emph{diff}}}}}$&\quad  \\
\\
difference of means & $\mu_1-\mu_2$ & $\bar{x}_1-\bar{x}_2$ & $\sqrt{\frac{s^2_1}{n_1}+\frac{s^2_2}{n_2}}$&
\end{tabular}
\vspace{1cm}

\noindent%
$\text{Chi-square test statistic} = \sum{\frac{(\text{observed} - \text{expected})^2}{\text{expected}}}$
\restoregeometry